<?xml version="1.0"?>
<rdf:RDF xmlns="https://w3id.org/cnr-ispc/ontology/branco#"
     xml:base="https://w3id.org/cnr-ispc/ontology/branco"
     xmlns:rdf="http://www.w3.org/1999/02/22-rdf-syntax-ns#"
     xmlns:owl="http://www.w3.org/2002/07/owl#"
     xmlns:xml="http://www.w3.org/XML/1998/namespace"
     xmlns:cidoc-crm="http://www.cidoc-crm.org/cidoc-crm/"
     xmlns:CRMdig="http://www.ics.forth.gr/isl/CRMdig/"
     xmlns:xsd="http://www.w3.org/2001/XMLSchema#"
     xmlns:rdfs="http://www.w3.org/2000/01/rdf-schema#"
     xmlns:hico="http://purl.org/emmedi/hico/"
     xmlns:branco_samod3="https://w3id.org/cnr-ispc/ontology/branco_samod3#"
     xmlns:dc="http://purl.org/dc/elements/1.1/"
     xmlns:cito="http://purl.org/spar/cito/">
    <owl:Ontology rdf:about="https://w3id.org/cnr-ispc/ontology/branco">
        <dc:rights rdf:resource="https://creativecommons.org/licenses/by/4.0/"/>
        <dc:title xml:lang="en">Branco - Brancacci Chapel Ontology</dc:title>
        <owl:versionInfo xml:lang="en">0.9.0</owl:versionInfo>
        <dc:creator xml:lang="en">Manuele Veggi, &quot;La Sapienza&quot; University of Rome - CNR ISPC
manuele.veggi@uniroma1.it</dc:creator>
	<dc:creator xml:lang="en">Ivana Cerato, CNR ISPC
ivana.cerato@cnr.it</dc:creator>
        <rdfs:comment xml:lang="en">&lt;b&gt;Branco&lt;/b&gt; (Brancacci Chapel Ontology) is an ontology for management of heterogeneous data and the reconstruction of historical sites and artworks which is based on the concept of intepretative unit, an adaptation of the concept of stratigraphic unit beyond the context of archeological excavation.

It is aligned with CIDOC-CRM (v.7.1.3) and CRMDig (v.3.2.1) and it uses specific classes of the Historical Context Ontology (HICO).

The ontology has been developed following the &lt;a href=&quot;https://essepuntato.it/samod/&quot;&gt;SAMOD protocol&lt;/a&gt;: see the reference &lt;a href=&quot;https://github.com/dhilab-fi/branco&quot;&gt;GitHub Repository&lt;/a&gt; for the material produced during the SAMOD iterations.

The ontology is a project of the CNR Institute of Heritage Science - Digital Heritage and Innovation Lab.

Author: Manuele Veggi (ontology engineer), Ivana Cerato (domain expert)
Contact point: Manuele Veggi, manuele.veggi@uniroma1.it</rdfs:comment>
    </owl:Ontology>
    


    <!-- 
    ///////////////////////////////////////////////////////////////////////////////////////
    //
    // Annotation properties
    //
    ///////////////////////////////////////////////////////////////////////////////////////
     -->

    


    <!-- http://purl.org/dc/elements/1.1/contributor -->

    <owl:AnnotationProperty rdf:about="http://purl.org/dc/elements/1.1/contributor"/>
    


    <!-- http://purl.org/dc/elements/1.1/creator -->

    <owl:AnnotationProperty rdf:about="http://purl.org/dc/elements/1.1/creator"/>
    


    <!-- http://purl.org/dc/elements/1.1/rights -->

    <owl:AnnotationProperty rdf:about="http://purl.org/dc/elements/1.1/rights"/>
    


    <!-- http://purl.org/dc/elements/1.1/title -->

    <owl:AnnotationProperty rdf:about="http://purl.org/dc/elements/1.1/title"/>
    


    <!-- 
    ///////////////////////////////////////////////////////////////////////////////////////
    //
    // Object Properties
    //
    ///////////////////////////////////////////////////////////////////////////////////////
     -->

    


    <!-- http://purl.org/emmedi/hico/hasInterpretationCriterion -->

    <owl:ObjectProperty rdf:about="http://purl.org/emmedi/hico/hasInterpretationCriterion">
        <rdfs:domain rdf:resource="http://purl.org/emmedi/hico/InterpretationAct"/>
        <rdfs:range rdf:resource="http://purl.org/emmedi/hico/InterpretationCriterion"/>
        <rdfs:comment xml:lang="en">A property relating an interpretation act to a criterion or type of source used to support the claim.</rdfs:comment>
        <rdfs:isDefinedBy rdf:resource="http://purl.org/emmedi/hico"/>
        <rdfs:label xml:lang="en">has interpretation criterion</rdfs:label>
    </owl:ObjectProperty>
    


    <!-- http://purl.org/spar/cito/cites -->

    <owl:ObjectProperty rdf:about="http://purl.org/spar/cito/cites">
        <rdfs:comment xml:lang="en">The citing entity cites the cited entity, either directly and explicitly (as in the reference list of a journal article), indirectly (e.g. by citing a more recent paper by the same group on the same topic), or implicitly (e.g. as in artistic quotations or parodies, or in cases of plagiarism).</rdfs:comment>
        <rdfs:isDefinedBy rdf:resource="http://purl.org/spar/cito"/>
    </owl:ObjectProperty>
    


    <!-- http://purl.org/spar/cito/citesAsEvidence -->

    <owl:ObjectProperty rdf:about="http://purl.org/spar/cito/citesAsEvidence">
        <rdfs:subPropertyOf rdf:resource="http://purl.org/spar/cito/cites"/>
        <rdfs:comment xml:lang="en">The citing entity cites the cited entity as source of factual evidence for statements it contains.

In the implementation of Branco, it allows to connect interpretations to a specific feature (&lt;code&gt;crm:E26_Physical_Feature&lt;/code&gt;) which supports an assertion of a property to the studied &lt;code&gt;crm:E18_Physical_Thing&lt;/code&gt;, as in style recognition (see individual :style).</rdfs:comment>
        <rdfs:isDefinedBy rdf:resource="http://purl.org/spar/cito"/>
        <rdfs:label xml:lang="en">cites as evidence</rdfs:label>
    </owl:ObjectProperty>
    


    <!-- http://www.cidoc-crm.org/cidoc-crm/P108_has_produced -->

    <owl:ObjectProperty rdf:about="http://www.cidoc-crm.org/cidoc-crm/P108_has_produced">
        <rdfs:subPropertyOf rdf:resource="http://www.cidoc-crm.org/cidoc-crm/P31_has_modified"/>
        <rdfs:subPropertyOf rdf:resource="http://www.cidoc-crm.org/cidoc-crm/P92_brought_into_existence"/>
        <owl:inverseOf rdf:resource="http://www.cidoc-crm.org/cidoc-crm/P108i_was_produced_by"/>
        <rdfs:domain rdf:resource="http://www.cidoc-crm.org/cidoc-crm/E12_Production"/>
        <rdfs:range rdf:resource="http://www.cidoc-crm.org/cidoc-crm/E24_Physical_Human-Made_Thing"/>
        <rdfs:comment xml:lang="en">This property identifies the instance of E24 Physical Human-Made Thing that came into existence as a result of the instance of E12 Production.
The identity of an instance of E24 Physical Human-Made Thing is not defined by its matter, but by its existence as a subject of documentation. An E12 Production can result in the creation of multiple instances of E24 Physical Human-Made Thing.</rdfs:comment>
        <rdfs:label xml:lang="fr">a produit</rdfs:label>
        <rdfs:label xml:lang="en">has produced</rdfs:label>
        <rdfs:label xml:lang="de">hat hergestellt</rdfs:label>
        <rdfs:label xml:lang="pt">produziu</rdfs:label>
        <rdfs:label xml:lang="el">παρήγαγε</rdfs:label>
        <rdfs:label xml:lang="ru">произвел</rdfs:label>
        <rdfs:label xml:lang="zh">已产生了</rdfs:label>
    </owl:ObjectProperty>
    


    <!-- http://www.cidoc-crm.org/cidoc-crm/P108i_was_produced_by -->

    <owl:ObjectProperty rdf:about="http://www.cidoc-crm.org/cidoc-crm/P108i_was_produced_by"/>
    


    <!-- http://www.cidoc-crm.org/cidoc-crm/P111_added -->

    <owl:ObjectProperty rdf:about="http://www.cidoc-crm.org/cidoc-crm/P111_added">
        <rdfs:subPropertyOf rdf:resource="http://www.cidoc-crm.org/cidoc-crm/P16_used_specific_object"/>
        <owl:inverseOf rdf:resource="http://www.cidoc-crm.org/cidoc-crm/P111i_was_added_by"/>
        <rdfs:domain rdf:resource="http://www.cidoc-crm.org/cidoc-crm/E79_Part_Addition"/>
        <rdfs:range rdf:resource="http://www.cidoc-crm.org/cidoc-crm/E18_Physical_Thing"/>
        <rdfs:comment xml:lang="en">This property identifies the instance of E18 Physical Thing that is added during an instance of E79 Part Addition activity.</rdfs:comment>
        <rdfs:label xml:lang="fr">a ajouté</rdfs:label>
        <rdfs:label xml:lang="en">added</rdfs:label>
        <rdfs:label xml:lang="pt">adicionou</rdfs:label>
        <rdfs:label xml:lang="de">fügte hinzu</rdfs:label>
        <rdfs:label xml:lang="el">προσέθεσε</rdfs:label>
        <rdfs:label xml:lang="ru">добавил</rdfs:label>
        <rdfs:label xml:lang="zh">增加了</rdfs:label>
    </owl:ObjectProperty>
    


    <!-- http://www.cidoc-crm.org/cidoc-crm/P111i_was_added_by -->

    <owl:ObjectProperty rdf:about="http://www.cidoc-crm.org/cidoc-crm/P111i_was_added_by"/>
    


    <!-- http://www.cidoc-crm.org/cidoc-crm/P113_removed -->

    <owl:ObjectProperty rdf:about="http://www.cidoc-crm.org/cidoc-crm/P113_removed">
        <rdfs:subPropertyOf rdf:resource="http://www.cidoc-crm.org/cidoc-crm/P12_occurred_in_the_presence_of"/>
        <owl:inverseOf rdf:resource="http://www.cidoc-crm.org/cidoc-crm/P113i_was_removed_by"/>
        <rdfs:domain rdf:resource="http://www.cidoc-crm.org/cidoc-crm/E80_Part_Removal"/>
        <rdfs:range rdf:resource="http://www.cidoc-crm.org/cidoc-crm/E18_Physical_Thing"/>
        <rdfs:comment xml:lang="en">This property identifies the instance of E18 Physical Thing that is removed during an instance of E80 Part Removal activity.</rdfs:comment>
        <rdfs:label xml:lang="fr">a retiré</rdfs:label>
        <rdfs:label xml:lang="de">entfernte</rdfs:label>
        <rdfs:label xml:lang="en">removed</rdfs:label>
        <rdfs:label xml:lang="pt">removeu</rdfs:label>
        <rdfs:label xml:lang="el">αφαίρεσε</rdfs:label>
        <rdfs:label xml:lang="ru">удален</rdfs:label>
        <rdfs:label xml:lang="zh">去除了</rdfs:label>
    </owl:ObjectProperty>
    


    <!-- http://www.cidoc-crm.org/cidoc-crm/P113i_was_removed_by -->

    <owl:ObjectProperty rdf:about="http://www.cidoc-crm.org/cidoc-crm/P113i_was_removed_by"/>
    


    <!-- http://www.cidoc-crm.org/cidoc-crm/P12_occurred_in_the_presence_of -->

    <owl:ObjectProperty rdf:about="http://www.cidoc-crm.org/cidoc-crm/P12_occurred_in_the_presence_of"/>
    


    <!-- http://www.cidoc-crm.org/cidoc-crm/P132_spatiotemporally_overlaps_with -->

    <owl:ObjectProperty rdf:about="http://www.cidoc-crm.org/cidoc-crm/P132_spatiotemporally_overlaps_with">
        <rdfs:domain rdf:resource="http://www.cidoc-crm.org/cidoc-crm/E5_Event"/>
        <rdfs:range rdf:resource="http://www.cidoc-crm.org/cidoc-crm/E5_Event"/>
    </owl:ObjectProperty>
    


    <!-- http://www.cidoc-crm.org/cidoc-crm/P13_destroyed -->

    <owl:ObjectProperty rdf:about="http://www.cidoc-crm.org/cidoc-crm/P13_destroyed">
        <rdfs:subPropertyOf rdf:resource="http://www.cidoc-crm.org/cidoc-crm/P93_took_out_of_existence"/>
        <owl:inverseOf rdf:resource="http://www.cidoc-crm.org/cidoc-crm/P13i_was_destroyed_by"/>
        <rdfs:domain rdf:resource="http://www.cidoc-crm.org/cidoc-crm/E6_Destruction"/>
        <rdfs:range rdf:resource="http://www.cidoc-crm.org/cidoc-crm/E18_Physical_Thing"/>
        <rdfs:comment xml:lang="en">This property links an instance of E6 Destruction to an instance of E18 Physical Thing that has been destroyed by it.
Destruction implies the end of an item’s life as a subject of cultural documentation – the physical matter of which the item was composed may in fact continue to exist. An instance of E6 Destruction may be contiguous with an instance of E12 Production that brings into existence a derived object composed partly of matter from the destroyed object.</rdfs:comment>
        <rdfs:label xml:lang="fr">a détruit</rdfs:label>
        <rdfs:label xml:lang="en">destroyed</rdfs:label>
        <rdfs:label xml:lang="pt">destruiu</rdfs:label>
        <rdfs:label xml:lang="de">zerstörte</rdfs:label>
        <rdfs:label xml:lang="el">κατέστρεψε</rdfs:label>
        <rdfs:label xml:lang="ru">уничтожил</rdfs:label>
        <rdfs:label xml:lang="zh">破坏了</rdfs:label>
    </owl:ObjectProperty>
    


    <!-- http://www.cidoc-crm.org/cidoc-crm/P13i_was_destroyed_by -->

    <owl:ObjectProperty rdf:about="http://www.cidoc-crm.org/cidoc-crm/P13i_was_destroyed_by"/>
    


    <!-- http://www.cidoc-crm.org/cidoc-crm/P140_assigned_attribute_to -->

    <owl:ObjectProperty rdf:about="http://www.cidoc-crm.org/cidoc-crm/P140_assigned_attribute_to">
        <owl:inverseOf rdf:resource="http://www.cidoc-crm.org/cidoc-crm/P140i_was_attributed_by"/>
        <rdfs:domain rdf:resource="http://www.cidoc-crm.org/cidoc-crm/E13_Attribute_Assignment"/>
        <rdfs:range rdf:resource="http://www.cidoc-crm.org/cidoc-crm/E1_CRM_Entity"/>
        <rdfs:comment xml:lang="en">This property associates an instance of E13 Attribute Assignment with the instance of E1 CRM Entity about which it made an attribution. The instance of E1 CRM Entity plays the role of the domain of the attribution.
The kind of attribution made should be documented using P177 assigned property of type (is type of property assigned).</rdfs:comment>
        <rdfs:label xml:lang="fr">a assigné l’attribut à</rdfs:label>
        <rdfs:label xml:lang="en">assigned attribute to</rdfs:label>
        <rdfs:label xml:lang="pt">atribuiu atributo para</rdfs:label>
        <rdfs:label xml:lang="de">wies Merkmal zu</rdfs:label>
        <rdfs:label xml:lang="el">απέδωσε ιδιότητα σε</rdfs:label>
        <rdfs:label xml:lang="ru">присвоил атрибут для</rdfs:label>
        <rdfs:label xml:lang="zh">分配属性于</rdfs:label>
    </owl:ObjectProperty>
    


    <!-- http://www.cidoc-crm.org/cidoc-crm/P140i_was_attributed_by -->

    <owl:ObjectProperty rdf:about="http://www.cidoc-crm.org/cidoc-crm/P140i_was_attributed_by"/>
    


    <!-- http://www.cidoc-crm.org/cidoc-crm/P141_assigned -->

    <owl:ObjectProperty rdf:about="http://www.cidoc-crm.org/cidoc-crm/P141_assigned">
        <rdfs:subPropertyOf rdf:resource="http://www.w3.org/2002/07/owl#topObjectProperty"/>
        <owl:inverseOf rdf:resource="http://www.cidoc-crm.org/cidoc-crm/P141i_was_assigned_by"/>
        <rdfs:domain rdf:resource="http://www.cidoc-crm.org/cidoc-crm/E13_Attribute_Assignment"/>
        <rdfs:range rdf:resource="http://www.cidoc-crm.org/cidoc-crm/E1_CRM_Entity"/>
        <rdfs:comment xml:lang="en">This property associates an instance of E13 Attribute Assignment with the instance of E1 CRM Entity used in the attribution. The instance of E1 CRM Entity here plays the role of the range of the attribution.
The kind of attribution made should be documented using P177 assigned property of type (is type of property assigned).</rdfs:comment>
        <rdfs:label xml:lang="fr">a attribué</rdfs:label>
        <rdfs:label xml:lang="en">assigned</rdfs:label>
        <rdfs:label xml:lang="pt">atribuiu</rdfs:label>
        <rdfs:label xml:lang="de">wies zu</rdfs:label>
        <rdfs:label xml:lang="el">απέδωσε</rdfs:label>
        <rdfs:label xml:lang="ru">присвоил</rdfs:label>
        <rdfs:label xml:lang="zh">分配</rdfs:label>
    </owl:ObjectProperty>
    


    <!-- http://www.cidoc-crm.org/cidoc-crm/P141i_was_assigned_by -->

    <owl:ObjectProperty rdf:about="http://www.cidoc-crm.org/cidoc-crm/P141i_was_assigned_by"/>
    


    <!-- http://www.cidoc-crm.org/cidoc-crm/P148_has_component -->

    <owl:ObjectProperty rdf:about="http://www.cidoc-crm.org/cidoc-crm/P148_has_component">
        <owl:inverseOf rdf:resource="http://www.cidoc-crm.org/cidoc-crm/P148i_is_component_of"/>
        <rdfs:domain rdf:resource="http://www.cidoc-crm.org/cidoc-crm/E89_Propositional_Object"/>
        <rdfs:range rdf:resource="http://www.cidoc-crm.org/cidoc-crm/E89_Propositional_Object"/>
        <rdfs:comment xml:lang="en">This property associates an instance of E89 Propositional Object with a structural part of it that is by itself an instance of E89 Propositional Object.
This property is transitive. This property is asymmetric.</rdfs:comment>
        <rdfs:label xml:lang="fr">a pour composant</rdfs:label>
        <rdfs:label xml:lang="en">has component</rdfs:label>
        <rdfs:label xml:lang="de">hat Bestandteil</rdfs:label>
        <rdfs:label xml:lang="zh">有组件</rdfs:label>
    </owl:ObjectProperty>
    


    <!-- http://www.cidoc-crm.org/cidoc-crm/P148i_is_component_of -->

    <owl:ObjectProperty rdf:about="http://www.cidoc-crm.org/cidoc-crm/P148i_is_component_of"/>
    


    <!-- http://www.cidoc-crm.org/cidoc-crm/P16_used_specific_object -->

    <owl:ObjectProperty rdf:about="http://www.cidoc-crm.org/cidoc-crm/P16_used_specific_object">
        <rdfs:subPropertyOf rdf:resource="http://www.cidoc-crm.org/cidoc-crm/P12_occurred_in_the_presence_of"/>
    </owl:ObjectProperty>
    


    <!-- http://www.cidoc-crm.org/cidoc-crm/P177_assigned_property_of_type -->

    <owl:ObjectProperty rdf:about="http://www.cidoc-crm.org/cidoc-crm/P177_assigned_property_of_type">
        <rdfs:subPropertyOf rdf:resource="http://www.cidoc-crm.org/cidoc-crm/P2_has_type"/>
        <owl:inverseOf rdf:resource="http://www.cidoc-crm.org/cidoc-crm/P177i_is_type_of_property_assigned"/>
        <rdfs:domain rdf:resource="http://www.cidoc-crm.org/cidoc-crm/E13_Attribute_Assignment"/>
        <rdfs:range rdf:resource="http://www.cidoc-crm.org/cidoc-crm/E55_Type"/>
        <rdfs:comment xml:lang="en">This property associates an instance of E13 Attribute Assignment with the type of property or relation that this assignment maintains to hold between the item to which it assigns an attribute and the attribute itself. Note that the properties defined by the CIDOC CRM also constitute instances of E55 Type themselves. The direction of the assigned property of type is understood to be from the attributed item (the range of property P140 assigned attribute to) to the attribute item (the range of the property P141 assigned). More than one property type may be assigned to hold between two items.
A comprehensive explanation about refining CIDOC CRM concepts by E55 Type is given in the section “About Types” in the section on “Specific Modelling Constructs” of this document.</rdfs:comment>
        <rdfs:label xml:lang="fr">a assigné le type de propriété</rdfs:label>
        <rdfs:label xml:lang="en">assigned property of type</rdfs:label>
    </owl:ObjectProperty>
    


    <!-- http://www.cidoc-crm.org/cidoc-crm/P177i_is_type_of_property_assigned -->

    <owl:ObjectProperty rdf:about="http://www.cidoc-crm.org/cidoc-crm/P177i_is_type_of_property_assigned"/>
    


    <!-- http://www.cidoc-crm.org/cidoc-crm/P1_is_identified_by -->

    <owl:ObjectProperty rdf:about="http://www.cidoc-crm.org/cidoc-crm/P1_is_identified_by"/>
    


    <!-- http://www.cidoc-crm.org/cidoc-crm/P2_has_type -->

    <owl:ObjectProperty rdf:about="http://www.cidoc-crm.org/cidoc-crm/P2_has_type">
        <rdfs:domain rdf:resource="http://www.cidoc-crm.org/cidoc-crm/E1_CRM_Entity"/>
        <rdfs:range rdf:resource="http://www.cidoc-crm.org/cidoc-crm/E55_Type"/>
    </owl:ObjectProperty>
    


    <!-- http://www.cidoc-crm.org/cidoc-crm/P31_has_modified -->

    <owl:ObjectProperty rdf:about="http://www.cidoc-crm.org/cidoc-crm/P31_has_modified">
        <rdfs:subPropertyOf rdf:resource="http://www.cidoc-crm.org/cidoc-crm/P12_occurred_in_the_presence_of"/>
        <owl:inverseOf rdf:resource="http://www.cidoc-crm.org/cidoc-crm/P31i_was_modified_by"/>
        <rdfs:domain rdf:resource="http://www.cidoc-crm.org/cidoc-crm/E11_Modification"/>
        <rdfs:range rdf:resource="http://www.cidoc-crm.org/cidoc-crm/E18_Physical_Thing"/>
        <rdfs:comment xml:lang="en">This property identifies the instance of E18 Physical Thing modified in an instance of E11 Modification.</rdfs:comment>
        <rdfs:label xml:lang="fr">a modifié</rdfs:label>
        <rdfs:label xml:lang="en">has modified</rdfs:label>
        <rdfs:label xml:lang="pt">modificou</rdfs:label>
        <rdfs:label xml:lang="de">veränderte</rdfs:label>
        <rdfs:label xml:lang="el">τροποποίησε</rdfs:label>
        <rdfs:label xml:lang="ru">изменил</rdfs:label>
        <rdfs:label xml:lang="zh">已更改</rdfs:label>
    </owl:ObjectProperty>
    


    <!-- http://www.cidoc-crm.org/cidoc-crm/P31i_was_modified_by -->

    <owl:ObjectProperty rdf:about="http://www.cidoc-crm.org/cidoc-crm/P31i_was_modified_by"/>
    


    <!-- http://www.cidoc-crm.org/cidoc-crm/P46_is_composed_of -->

    <owl:ObjectProperty rdf:about="http://www.cidoc-crm.org/cidoc-crm/P46_is_composed_of">
        <owl:inverseOf rdf:resource="http://www.cidoc-crm.org/cidoc-crm/P46i_forms_part_of"/>
        <rdfs:domain rdf:resource="http://www.cidoc-crm.org/cidoc-crm/E18_Physical_Thing"/>
        <rdfs:range rdf:resource="http://www.cidoc-crm.org/cidoc-crm/E18_Physical_Thing"/>
        <rdfs:comment xml:lang="en">This property associates an instance of E18 Physical Thing with another instance of Physical Thing that forms part of it. The spatial extent of the composing part is included in the spatial extent of the whole.
Component elements, since they are themselves instances of E18 Physical Thing, may be further analysed into sub-components, thereby creating a hierarchy of part decomposition. An instance of E18 Physical Thing may be shared between multiple wholes, for example two buildings may share a common wall. This property does not specify when and for how long a component element resided in the respective whole. If a component is not part of a whole from the beginning of existence or until the end of existence of the whole, the classes E79 Part Addition and E90 Part Removal can be used to document when a component became part of a particular whole and/or when it stopped being a part of it. For the time-span of being part of the respective whole, the component is completely contained in the place the whole occupies.
This property is intended to describe specific components that are individually documented, rather than general aspects. Overall descriptions of the structure of an instance of E18 Physical Thing are captured by the P3 has note property.
The instances of E57 Material of which an instance of E18 Physical Thing is composed should be documented using P45 consists of (is incorporated in).
This property is transitive and asymmetric.</rdfs:comment>
        <rdfs:label xml:lang="fr">est composé de</rdfs:label>
        <rdfs:label xml:lang="en">is composed of</rdfs:label>
        <rdfs:label xml:lang="de">ist zusammengesetzt aus</rdfs:label>
        <rdfs:label xml:lang="pt">é composto de</rdfs:label>
        <rdfs:label xml:lang="el">αποτελείται από</rdfs:label>
        <rdfs:label xml:lang="ru">составлен из</rdfs:label>
        <rdfs:label xml:lang="zh">组成成分是</rdfs:label>
    </owl:ObjectProperty>
    


    <!-- http://www.cidoc-crm.org/cidoc-crm/P46i_forms_part_of -->

    <owl:ObjectProperty rdf:about="http://www.cidoc-crm.org/cidoc-crm/P46i_forms_part_of"/>
    


    <!-- http://www.cidoc-crm.org/cidoc-crm/P48_has_preferred_identifier -->

    <owl:ObjectProperty rdf:about="http://www.cidoc-crm.org/cidoc-crm/P48_has_preferred_identifier">
        <rdfs:subPropertyOf rdf:resource="http://www.cidoc-crm.org/cidoc-crm/P1_is_identified_by"/>
        <owl:inverseOf rdf:resource="http://www.cidoc-crm.org/cidoc-crm/P48i_is_preferred_identifier_of"/>
        <rdfs:domain rdf:resource="http://www.cidoc-crm.org/cidoc-crm/E1_CRM_Entity"/>
    </owl:ObjectProperty>
    


    <!-- http://www.cidoc-crm.org/cidoc-crm/P48i_is_preferred_identifier_of -->

    <owl:ObjectProperty rdf:about="http://www.cidoc-crm.org/cidoc-crm/P48i_is_preferred_identifier_of"/>
    


    <!-- http://www.cidoc-crm.org/cidoc-crm/P67_refers_to -->

    <owl:ObjectProperty rdf:about="http://www.cidoc-crm.org/cidoc-crm/P67_refers_to">
        <owl:inverseOf rdf:resource="http://www.cidoc-crm.org/cidoc-crm/P67i_is_referred_to_by"/>
        <rdfs:domain rdf:resource="http://www.cidoc-crm.org/cidoc-crm/E89_Propositional_Object"/>
        <rdfs:range rdf:resource="http://www.cidoc-crm.org/cidoc-crm/E1_CRM_Entity"/>
        <rdfs:comment xml:lang="en">This property documents that an instance of E89 Propositional Object makes a statement about an instance of E1 CRM Entity. P67 refers to (is referred to by) has the P67.1 has type link to an instance of E55 Type. This is intended to allow a more detailed description of the type of reference. This differs from P129 is about (is subject of), which describes the primary subject or subjects of the instance of E89 Propositional Object.</rdfs:comment>
        <rdfs:label xml:lang="pt">referencia</rdfs:label>
        <rdfs:label xml:lang="en">refers to</rdfs:label>
        <rdfs:label xml:lang="fr">renvoie à</rdfs:label>
        <rdfs:label xml:lang="de">verweist auf</rdfs:label>
        <rdfs:label xml:lang="el">αναφέρεται σε</rdfs:label>
        <rdfs:label xml:lang="ru">ссылается на</rdfs:label>
        <rdfs:label xml:lang="zh">涉及</rdfs:label>
    </owl:ObjectProperty>
    


    <!-- http://www.cidoc-crm.org/cidoc-crm/P67i_is_referred_to_by -->

    <owl:ObjectProperty rdf:about="http://www.cidoc-crm.org/cidoc-crm/P67i_is_referred_to_by"/>
    


    <!-- http://www.cidoc-crm.org/cidoc-crm/P91i_is_unit_of -->

    <owl:ObjectProperty rdf:about="http://www.cidoc-crm.org/cidoc-crm/P91i_is_unit_of"/>
    


    <!-- http://www.cidoc-crm.org/cidoc-crm/P92_brought_into_existence -->

    <owl:ObjectProperty rdf:about="http://www.cidoc-crm.org/cidoc-crm/P92_brought_into_existence"/>
    


    <!-- http://www.cidoc-crm.org/cidoc-crm/P93_took_out_of_existence -->

    <owl:ObjectProperty rdf:about="http://www.cidoc-crm.org/cidoc-crm/P93_took_out_of_existence"/>
    


    <!-- http://www.ics.forth.gr/isl/CRMdig/L11_had_output -->

    <owl:ObjectProperty rdf:about="http://www.ics.forth.gr/isl/CRMdig/L11_had_output">
        <rdfs:domain rdf:resource="http://www.ics.forth.gr/isl/CRMdig/D7_Digital_Machine_Event"/>
        <rdfs:range rdf:resource="http://www.ics.forth.gr/isl/CRMdig/D1_Digital_Object"/>
        <rdfs:comment xml:lang="en">This property associates an instance of D7 Digital Machine Event with an instance of D1 Digital Object
 which is the output of the activity.  
This property is a specialisation of P94 has created (was created by).</rdfs:comment>
    </owl:ObjectProperty>
    


    <!-- http://www.ics.forth.gr/isl/CRMdig/L1_digitized -->

    <owl:ObjectProperty rdf:about="http://www.ics.forth.gr/isl/CRMdig/L1_digitized">
        <rdfs:domain rdf:resource="http://www.ics.forth.gr/isl/CRMdig/D2_Digitization_Process"/>
        <rdfs:range rdf:resource="http://www.cidoc-crm.org/cidoc-crm/E18_Physical_Thing"/>
        <rdfs:comment xml:lang="en">This property associates an instance of D2 Digitization Process with an instance of E18 Physical Thing which is a material thing.  
This property is a specialisation of P39 measured (was measured by).
</rdfs:comment>
    </owl:ObjectProperty>
    


    <!-- http://www.ics.forth.gr/isl/CRMdig/L43i_is_annotated_by -->

    <owl:ObjectProperty rdf:about="http://www.ics.forth.gr/isl/CRMdig/L43i_is_annotated_by">
        <rdfs:domain rdf:resource="http://www.cidoc-crm.org/cidoc-crm/E1_CRM_Entity"/>
        <rdfs:range rdf:resource="http://www.ics.forth.gr/isl/CRMdig/D29_Annotation_Object"/>
    </owl:ObjectProperty>
    


    <!-- https://w3id.org/cnr-ispc/ontology/branco#covers -->

    <owl:ObjectProperty rdf:about="https://w3id.org/cnr-ispc/ontology/branco#covers">
        <rdfs:domain rdf:resource="https://w3id.org/cnr-ispc/ontology/branco#CladdingUnit"/>
        <rdfs:range rdf:resource="https://w3id.org/cnr-ispc/ontology/branco#StructuralUnit"/>
        <rdfs:comment xml:lang="en">This property connects a cladding unit to its reference structural unit, e.g. the production of a fresco decoration on a wall.</rdfs:comment>
        <rdfs:isDefinedBy rdf:resource="https://w3id.org/cnr-ispc/ontology/branco#"/>
    </owl:ObjectProperty>
    


    <!-- https://w3id.org/cnr-ispc/ontology/branco#hasNode -->

    <owl:ObjectProperty rdf:about="https://w3id.org/cnr-ispc/ontology/branco#hasNode">
        <rdfs:domain rdf:resource="http://www.ics.forth.gr/isl/CRMdig/D9_Data_Object"/>
        <rdfs:range rdf:resource="https://w3id.org/cnr-ispc/ontology/branco#SemanticNode"/>
        <rdfs:comment xml:lang="en">This property connects a digital object to the one or more semantic nodes that annotates it</rdfs:comment>
        <rdfs:isDefinedBy rdf:resource="https://w3id.org/cnr-ispc/ontology/branco#"/>
    </owl:ObjectProperty>
    


    <!-- https://w3id.org/cnr-ispc/ontology/branco#involves -->

    <owl:ObjectProperty rdf:about="https://w3id.org/cnr-ispc/ontology/branco#involves">
        <rdfs:domain rdf:resource="https://w3id.org/cnr-ispc/ontology/branco#InterpretativeUnit"/>
        <rdfs:range rdf:resource="http://www.cidoc-crm.org/cidoc-crm/E18_Physical_Thing"/>
        <rdfs:comment xml:lang="en">This property further describes an interpretative unit: it allows to directly link it with the physical thing that is undergoing a process of &lt;code&gt;crm:E6_Destruction&lt;/code&gt; or &lt;code&gt;crm:E11_Modification&lt;/code&gt;</rdfs:comment>
        <rdfs:isDefinedBy rdf:resource="https://w3id.org/cnr-ispc/ontology/branco#"/>
    </owl:ObjectProperty>
    


    <!-- https://w3id.org/cnr-ispc/ontology/branco#models -->

    <owl:ObjectProperty rdf:about="https://w3id.org/cnr-ispc/ontology/branco#models">
        <rdfs:domain rdf:resource="https://w3id.org/cnr-ispc/ontology/branco#InterpretativeUnit"/>
        <rdfs:range>
            <owl:Class>
                <owl:unionOf rdf:parseType="Collection">
                    <rdf:Description rdf:about="http://www.cidoc-crm.org/cidoc-crm/E11_Modification"/>
                    <rdf:Description rdf:about="http://www.cidoc-crm.org/cidoc-crm/E6_Destruction"/>
                </owl:unionOf>
            </owl:Class>
        </rdfs:range>
        <rdfs:comment xml:lang="en">Interpretative units model events of type &lt;code&gt;crm:E6_Destruction&lt;/code&gt; or &lt;code&gt;crm:E11_Modification&lt;/code&gt; on a physical thing: this property allows to link an interpretative unit to one of these processes</rdfs:comment>
        <rdfs:isDefinedBy rdf:resource="https://w3id.org/cnr-ispc/ontology/branco#"/>
    </owl:ObjectProperty>
    


    <!-- https://w3id.org/cnr-ispc/ontology/branco#providesComparisonWith -->

    <owl:ObjectProperty rdf:about="https://w3id.org/cnr-ispc/ontology/branco#providesComparisonWith">
        <rdfs:subPropertyOf rdf:resource="http://purl.org/spar/cito/cites"/>
        <rdfs:domain rdf:resource="https://w3id.org/cnr-ispc/ontology/branco#Interpretation"/>
        <rdfs:range rdf:resource="http://www.cidoc-crm.org/cidoc-crm/E18_Physical_Thing"/>
        <rdfs:comment xml:lang="en">Interpretations may be based on a comparison with other relevant artwork or sites displaying similar features with the current case study. This properties associates the interpretation with the object of comparison.</rdfs:comment>
        <rdfs:isDefinedBy rdf:resource="https://w3id.org/cnr-ispc/ontology/branco#"/>
    </owl:ObjectProperty>
    


    <!-- 
    ///////////////////////////////////////////////////////////////////////////////////////
    //
    // Data properties
    //
    ///////////////////////////////////////////////////////////////////////////////////////
     -->

    


    <!-- https://w3id.org/cnr-ispc/ontology/branco#hasChronologicalOrder -->

    <owl:DatatypeProperty rdf:about="https://w3id.org/cnr-ispc/ontology/branco#hasChronologicalOrder">
        <rdfs:domain rdf:resource="https://w3id.org/cnr-ispc/ontology/branco#InterpretativeUnit"/>
        <rdfs:range rdf:resource="http://www.w3.org/2001/XMLSchema#integer"/>
        <rdfs:comment xml:lang="en">Interpretative units models a series of events: as a result they may be organised chronologically thanks to this data property</rdfs:comment>
        <rdfs:isDefinedBy rdf:resource="https://w3id.org/cnr-ispc/ontology/branco#"/>
    </owl:DatatypeProperty>
    


    <!-- 
    ///////////////////////////////////////////////////////////////////////////////////////
    //
    // Classes
    //
    ///////////////////////////////////////////////////////////////////////////////////////
     -->

    


    <!-- http://purl.org/emmedi/hico/InterpretationAct -->

    <owl:Class rdf:about="http://purl.org/emmedi/hico/InterpretationAct">
        <rdfs:subClassOf rdf:resource="http://www.w3.org/ns/prov#Activity"/>
        <rdfs:subClassOf>
            <owl:Restriction>
                <owl:onProperty rdf:resource="http://purl.org/emmedi/hico/hasInterpretationCriterion"/>
                <owl:someValuesFrom rdf:resource="http://purl.org/emmedi/hico/InterpretationCriterion"/>
            </owl:Restriction>
        </rdfs:subClassOf>
    </owl:Class>
    


    <!-- http://purl.org/emmedi/hico/InterpretationCriterion -->

    <owl:Class rdf:about="http://purl.org/emmedi/hico/InterpretationCriterion">
        <rdfs:subClassOf rdf:resource="http://www.w3.org/2002/07/owl#Thing"/>
        <rdfs:comment xml:lang="en">The criterion or type of source used by an agent to support an interpretation act, such as bibliography, verbal communication, etc. </rdfs:comment>
        <rdfs:isDefinedBy rdf:resource="http://purl.org/emmedi/hico"/>
        <rdfs:label xml:lang="en">Interpretation Criterion</rdfs:label>
    </owl:Class>
    


    <!-- http://www.cidoc-crm.org/cidoc-crm/E11_Modification -->

    <owl:Class rdf:about="http://www.cidoc-crm.org/cidoc-crm/E11_Modification">
        <rdfs:subClassOf rdf:resource="http://www.cidoc-crm.org/cidoc-crm/E7_Activity"/>
        <owl:disjointWith rdf:resource="http://www.cidoc-crm.org/cidoc-crm/E6_Destruction"/>
        <rdfs:comment xml:lang="en">This class comprises instances of E7 Activity that are undertaken to create, alter or change instances of E24 Physical Human-Made Thing.
This class includes the production of an item from raw materials and other so far undocumented objects. It also includes the conservation treatment of an object.
Since the distinction between modification and production is not always clear, modification is regarded as the more generally applicable concept. This implies that some items may be consumed or destroyed in an instance of E11 Modification, and that others may be produced as a result of it. An event should also be documented using an instance of E81 Transformation if it results in the destruction of one or more objects and the simultaneous production of others using parts or material from the originals. In this case, the new items have separate identities.
An activity undertaken on an object which was designed to alter it, but which, in fact, it did not in any seemingly significant way (such as the application of a solvent during conservation which failed to dissolve any part of the object), is still considered as an instance of E11 Modification. Typically, any such activity will leave at least forensic traces of evidence on the object.
If the instance of E29 Design or Procedure utilized for the modification prescribes the use of specific materials, they should be documented using property P68 foresees use of (use foreseen by): E57 Material of E29 Design or Procedure, rather than via P126 employed (was employed in): E57 Material.</rdfs:comment>
        <rdfs:label xml:lang="de">Bearbeitung</rdfs:label>
        <rdfs:label xml:lang="en">Modification</rdfs:label>
        <rdfs:label xml:lang="fr">Modification</rdfs:label>
        <rdfs:label xml:lang="pt">Modificação</rdfs:label>
        <rdfs:label xml:lang="el">Τροποποίηση</rdfs:label>
        <rdfs:label xml:lang="ru">Событие Изменения</rdfs:label>
        <rdfs:label xml:lang="zh">修改</rdfs:label>
    </owl:Class>
    


    <!-- http://www.cidoc-crm.org/cidoc-crm/E12_Production -->

    <owl:Class rdf:about="http://www.cidoc-crm.org/cidoc-crm/E12_Production">
        <rdfs:subClassOf rdf:resource="http://www.cidoc-crm.org/cidoc-crm/E11_Modification"/>
        <rdfs:subClassOf rdf:resource="http://www.cidoc-crm.org/cidoc-crm/E63_Beginning_of_Existence"/>
        <rdfs:comment xml:lang="en">This class comprises activities that are designed to, and succeed in, creating one or more new items.
It specializes the notion of modification into production. The decision as to whether or not an object is regarded as new is context sensitive. Normally, items are considered “new” if there is no obvious overall similarity between them and the consumed items and material used in their production. In other cases, an item is considered “new” because it becomes relevant to documentation by a modification. For example, the scribbling of a name on a potsherd may make it a voting token. The original potsherd may not be worth documenting, in contrast to the inscribed one.
This entity can be collective: the printing of a thousand books, for example, would normally be considered a single event.
An event should also be documented using an instance of E81 Transformation if it results in the destruction of one or more objects and the simultaneous production of others using parts or material from the originals. In this case, the new items have separate identities and matter is preserved, but identity is not.</rdfs:comment>
        <rdfs:label xml:lang="de">Herstellung</rdfs:label>
        <rdfs:label xml:lang="en">Production</rdfs:label>
        <rdfs:label xml:lang="fr">Production</rdfs:label>
        <rdfs:label xml:lang="pt">Produção</rdfs:label>
        <rdfs:label xml:lang="el">Παραγωγή</rdfs:label>
        <rdfs:label xml:lang="ru">Событие Производства</rdfs:label>
        <rdfs:label xml:lang="zh">生产</rdfs:label>
    </owl:Class>
    


    <!-- http://www.cidoc-crm.org/cidoc-crm/E13_Attribute_Assignment -->

    <owl:Class rdf:about="http://www.cidoc-crm.org/cidoc-crm/E13_Attribute_Assignment">
        <rdfs:subClassOf rdf:resource="http://www.cidoc-crm.org/cidoc-crm/E7_Activity"/>
    </owl:Class>
    


    <!-- http://www.cidoc-crm.org/cidoc-crm/E18_Physical_Thing -->

    <owl:Class rdf:about="http://www.cidoc-crm.org/cidoc-crm/E18_Physical_Thing">
        <rdfs:subClassOf rdf:resource="http://www.cidoc-crm.org/cidoc-crm/E72_Legal_Object"/>
        <rdfs:comment xml:lang="en">This class comprises all persistent physical items with a relatively stable form, human-made or natural.
Depending on the existence of natural boundaries of such things, the CIDOC CRM distinguishes the instances of E19 Physical Object from instances of E26 Physical Feature, such as holes, rivers, pieces of land, etc. Most instances of E19 Physical Object can be moved (if not too heavy), whereas features are integral to the surrounding matter.
An instance of E18 Physical Thing occupies not only a particular geometric space at any instant of its existence, but in the course of its existence it also forms a trajectory through spacetime, which occupies a real, that is phenomenal, volume in spacetime. We include in the occupied space the space filled by the matter of the physical thing and all its inner spaces, such as the interior of a box. For the purpose of more detailed descriptions of the presence of an instance of E18 Physical Thing in space and time it can be associated with its specific instance of E92 Spacetime Volume by the property P196 defines (is defined by).
The CIDOC CRM is generally not concerned with amounts of matter in fluid or gaseous states, as long as they are not confined in an identifiable way for an identifiable minimal time-span.</rdfs:comment>
        <rdfs:label xml:lang="fr">Chose matérielle</rdfs:label>
        <rdfs:label xml:lang="pt">Coisa Material</rdfs:label>
        <rdfs:label xml:lang="de">Materielles</rdfs:label>
        <rdfs:label xml:lang="en">Physical Thing</rdfs:label>
        <rdfs:label xml:lang="el">Υλικό Πράγμα</rdfs:label>
        <rdfs:label xml:lang="ru">Физическая Вещь</rdfs:label>
        <rdfs:label xml:lang="zh">实物</rdfs:label>
    </owl:Class>
    


    <!-- http://www.cidoc-crm.org/cidoc-crm/E1_CRM_Entity -->

    <owl:Class rdf:about="http://www.cidoc-crm.org/cidoc-crm/E1_CRM_Entity"/>
    


    <!-- http://www.cidoc-crm.org/cidoc-crm/E24_Physical_Human-Made_Thing -->

    <owl:Class rdf:about="http://www.cidoc-crm.org/cidoc-crm/E24_Physical_Human-Made_Thing">
        <rdfs:subClassOf rdf:resource="http://www.cidoc-crm.org/cidoc-crm/E18_Physical_Thing"/>
    </owl:Class>
    


    <!-- http://www.cidoc-crm.org/cidoc-crm/E26_Physical_Feature -->

    <owl:Class rdf:about="http://www.cidoc-crm.org/cidoc-crm/E26_Physical_Feature">
        <rdfs:subClassOf rdf:resource="http://www.cidoc-crm.org/cidoc-crm/E18_Physical_Thing"/>
        <rdfs:comment xml:lang="en">This class comprises identifiable features that are physically attached in an integral way to particular physical objects.
Instances of E26 Physical Feature share many of the attributes of instances of E19 Physical Object. They may have a one-dimensional, two-dimensional, or three-dimensional geometric extent, but there are no natural borders that separate them completely in an objective way from the carrier objects. For example, a doorway is a feature but the door itself, being attached by hinges, is not.
Instances of E26 Physical Feature can be features in a narrower sense, such as scratches, holes, reliefs, surface colours, reflection zones in an opal crystal or a density change in a piece of wood. In the wider sense, they are portions of particular objects with partially imaginary borders, such as the core of the Earth, an area of property on the surface of the Earth, a landscape or the head of a contiguous marble statue. They can be measured and dated, and it is sometimes possible to state who or what is or was responsible for them. They cannot be separated from the carrier object, but a segment of the carrier object may be identified (or sometimes removed) carrying the complete feature.
This definition coincides with the definition of “fiat objects”, with the exception of aggregates of “bona fide objects” (Smith &amp;amp; Varzi, 2000).</rdfs:comment>
        <rdfs:label xml:lang="pt">Característica Material</rdfs:label>
        <rdfs:label xml:lang="fr">Caractéristique physique</rdfs:label>
        <rdfs:label xml:lang="de">Materielles Merkmal</rdfs:label>
        <rdfs:label xml:lang="en">Physical Feature</rdfs:label>
        <rdfs:label xml:lang="el">Υλικό Μόρφωμα</rdfs:label>
        <rdfs:label xml:lang="ru">Физический Признак</rdfs:label>
        <rdfs:label xml:lang="zh">物理特征</rdfs:label>
    </owl:Class>
    


    <!-- http://www.cidoc-crm.org/cidoc-crm/E28_Conceptual_Object -->

    <owl:Class rdf:about="http://www.cidoc-crm.org/cidoc-crm/E28_Conceptual_Object">
        <rdfs:subClassOf rdf:resource="http://www.cidoc-crm.org/cidoc-crm/E28_Conceptual_Object"/>
    </owl:Class>
    


    <!-- http://www.cidoc-crm.org/cidoc-crm/E4_Period -->

    <owl:Class rdf:about="http://www.cidoc-crm.org/cidoc-crm/E4_Period"/>
    


    <!-- http://www.cidoc-crm.org/cidoc-crm/E54_Dimension -->

    <owl:Class rdf:about="http://www.cidoc-crm.org/cidoc-crm/E54_Dimension">
        <rdfs:subClassOf rdf:resource="http://www.cidoc-crm.org/cidoc-crm/E1_CRM_Entity"/>
    </owl:Class>
    


    <!-- http://www.cidoc-crm.org/cidoc-crm/E55_Type -->

    <owl:Class rdf:about="http://www.cidoc-crm.org/cidoc-crm/E55_Type">
        <rdfs:subClassOf rdf:resource="http://www.cidoc-crm.org/cidoc-crm/E28_Conceptual_Object"/>
        <rdfs:subClassOf rdf:resource="http://www.cidoc-crm.org/cidoc-crm/E55_Type"/>
        <rdfs:comment xml:lang="en">This class comprises concepts denoted by terms from thesauri and controlled vocabularies used to characterize and classify instances of CIDOC CRM classes. Instances of E55 Type represent concepts, in contrast to instances of E41 Appellation which are used to name instances of CIDOC CRM classes.
E55 Type provides an interface to domain specific ontologies and thesauri. These can be represented in the CIDOC CRM as subclasses of E55 Type, forming hierarchies of terms, i.e. instances of E55 Type linked via P127 has broader term (has narrower term): E55 Type. Such hierarchies may be extended with additional properties.</rdfs:comment>
        <rdfs:label xml:lang="pt">Tipo</rdfs:label>
        <rdfs:label xml:lang="en">Type</rdfs:label>
        <rdfs:label xml:lang="fr">Type</rdfs:label>
        <rdfs:label xml:lang="de">Typus</rdfs:label>
        <rdfs:label xml:lang="el">Τύπος</rdfs:label>
        <rdfs:label xml:lang="ru">Тип</rdfs:label>
        <rdfs:label xml:lang="zh">类型</rdfs:label>
    </owl:Class>
    


    <!-- http://www.cidoc-crm.org/cidoc-crm/E5_Event -->

    <owl:Class rdf:about="http://www.cidoc-crm.org/cidoc-crm/E5_Event">
        <rdfs:subClassOf rdf:resource="http://www.cidoc-crm.org/cidoc-crm/E4_Period"/>
    </owl:Class>
    


    <!-- http://www.cidoc-crm.org/cidoc-crm/E63_Beginning_of_Existence -->

    <owl:Class rdf:about="http://www.cidoc-crm.org/cidoc-crm/E63_Beginning_of_Existence">
        <rdfs:subClassOf rdf:resource="http://www.cidoc-crm.org/cidoc-crm/E5_Event"/>
    </owl:Class>
    


    <!-- http://www.cidoc-crm.org/cidoc-crm/E64_End_of_Existence -->

    <owl:Class rdf:about="http://www.cidoc-crm.org/cidoc-crm/E64_End_of_Existence">
        <rdfs:subClassOf rdf:resource="http://www.cidoc-crm.org/cidoc-crm/E5_Event"/>
    </owl:Class>
    


    <!-- http://www.cidoc-crm.org/cidoc-crm/E6_Destruction -->

    <owl:Class rdf:about="http://www.cidoc-crm.org/cidoc-crm/E6_Destruction">
        <rdfs:subClassOf rdf:resource="http://www.cidoc-crm.org/cidoc-crm/E64_End_of_Existence"/>
        <rdfs:comment xml:lang="en">This class comprises events that destroy one or more instances of E18 Physical Thing, such that they lose their identity as the subjects of documentation.
Some destruction events are intentional, while others are independent of human activity. Intentional destruction can be documented by classifying the event as both an instance of E6 Destruction and of E7 Activity.
The decision to document an object as destroyed, transformed, or modified is context-sensitive:
1. If the matter remaining from the destruction is not documented, the event is modelled solely as an instance of E6 Destruction.
2. An event should also be documented using E81 Transformation if it results in the destruction of one or more objects and the simultaneous production of others using parts or material from the original. In this case, the new items have separate identities. Matter is preserved, but identity is not.
3. When the initial identity of the changed instance of E18 Physical Thing is preserved, the event should be documented as an instance of E11 Modification.</rdfs:comment>
        <rdfs:label xml:lang="en">Destruction</rdfs:label>
        <rdfs:label xml:lang="fr">Destruction</rdfs:label>
        <rdfs:label xml:lang="pt">Destruição</rdfs:label>
        <rdfs:label xml:lang="de">Zerstörung</rdfs:label>
        <rdfs:label xml:lang="el">Καταστροφή</rdfs:label>
        <rdfs:label xml:lang="ru">Разрушение</rdfs:label>
        <rdfs:label xml:lang="zh">破坏</rdfs:label>
    </owl:Class>
    


    <!-- http://www.cidoc-crm.org/cidoc-crm/E72_Legal_Object -->

    <owl:Class rdf:about="http://www.cidoc-crm.org/cidoc-crm/E72_Legal_Object"/>
    


    <!-- http://www.cidoc-crm.org/cidoc-crm/E79_Part_Addition -->

    <owl:Class rdf:about="http://www.cidoc-crm.org/cidoc-crm/E79_Part_Addition">
        <rdfs:subClassOf rdf:resource="http://www.cidoc-crm.org/cidoc-crm/E11_Modification"/>
        <rdfs:comment xml:lang="en">This class comprises activities that result in an instance of E18 Physical Thing being increased, enlarged, or augmented by the addition of a part.
Typical scenarios include the attachment of an accessory, the integration of a component, the addition of an element to an aggregate object, or the accessioning of an object into a curated instance of E78 Curated Holding. Both the E18 Physical Thing being augmented and the E18 Physical Thing that is being added are treated as separate identifiable wholes prior to the instance of E79 Part Addition. Following the addition of parts, the resulting assemblages are treated objectively as single identifiable wholes, made up of constituent or component parts bound together either physically (for example the engine becoming a part of the car), or by sharing a common purpose (such as the 32 chess pieces that make up a chess set). This class of activities forms a basis for reasoning about the history and continuity of identity of objects that are integrated into other objects over time, such as precious gemstones being repeatedly incorporated into different items of jewellery, or cultural artefacts being added to different museum instances of E78 Curated Holding over their lifespan.</rdfs:comment>
        <rdfs:label xml:lang="pt">Adição de Parte</rdfs:label>
        <rdfs:label xml:lang="fr">Ajout d&apos;élément</rdfs:label>
        <rdfs:label xml:lang="en">Part Addition</rdfs:label>
        <rdfs:label xml:lang="de">Teilhinzufügung</rdfs:label>
        <rdfs:label xml:lang="el">Προσθήκη Μερών</rdfs:label>
        <rdfs:label xml:lang="ru">Добавление Части</rdfs:label>
        <rdfs:label xml:lang="zh">部分增加</rdfs:label>
    </owl:Class>
    


    <!-- http://www.cidoc-crm.org/cidoc-crm/E7_Activity -->

    <owl:Class rdf:about="http://www.cidoc-crm.org/cidoc-crm/E7_Activity">
        <rdfs:subClassOf rdf:resource="http://www.cidoc-crm.org/cidoc-crm/E5_Event"/>
    </owl:Class>
    


    <!-- http://www.cidoc-crm.org/cidoc-crm/E80_Part_Removal -->

    <owl:Class rdf:about="http://www.cidoc-crm.org/cidoc-crm/E80_Part_Removal">
        <rdfs:subClassOf rdf:resource="http://www.cidoc-crm.org/cidoc-crm/E11_Modification"/>
        <rdfs:comment xml:lang="en">This class comprises the activities that result in an instance of E18 Physical Thing being decreased by the removal of a part.
Typical scenarios include the detachment of an accessory, the removal of a component or part of a composite object, or the deaccessioning of an object from a curated collection, an instance of E78 Curated Holding. If the instance of E80 Part Removal results in the total decomposition of the original object into pieces, such that the whole ceases to exist, the activity should instead be modelled as an instance of E81 Transformation, i.e. a simultaneous destruction and production. In cases where the part removed has no discernible identity prior to its removal but does have an identity subsequent to its removal, the activity should be modelled as both an instance of E80 Part Removal and E12 Production. This class of activities forms a basis for reasoning about the history, and continuity of identity over time, of objects that are removed from other objects, such as precious gemstones being extracted from different items of jewellery, or cultural artifacts being deaccessioned from different museum collections over their lifespan.</rdfs:comment>
        <rdfs:label xml:lang="en">Part Removal</rdfs:label>
        <rdfs:label xml:lang="pt">Remoção de Parte</rdfs:label>
        <rdfs:label xml:lang="fr">Retrait d&apos;élément</rdfs:label>
        <rdfs:label xml:lang="de">Teilentfernung</rdfs:label>
        <rdfs:label xml:lang="el">Αφαίρεση Μερών</rdfs:label>
        <rdfs:label xml:lang="ru">Удаление Части</rdfs:label>
        <rdfs:label xml:lang="zh">部分去除</rdfs:label>
    </owl:Class>
    


    <!-- http://www.cidoc-crm.org/cidoc-crm/E89_Propositional_Object -->

    <owl:Class rdf:about="http://www.cidoc-crm.org/cidoc-crm/E89_Propositional_Object">
        <rdfs:subClassOf rdf:resource="http://www.cidoc-crm.org/cidoc-crm/E28_Conceptual_Object"/>
    </owl:Class>
    


    <!-- http://www.ics.forth.gr/isl/CRMdig/D11_Digital_Measurement_Event -->

    <owl:Class rdf:about="http://www.ics.forth.gr/isl/CRMdig/D11_Digital_Measurement_Event"/>
    


    <!-- http://www.ics.forth.gr/isl/CRMdig/D1_Digital_Object -->

    <owl:Class rdf:about="http://www.ics.forth.gr/isl/CRMdig/D1_Digital_Object"/>
    


    <!-- http://www.ics.forth.gr/isl/CRMdig/D29_Annotation_Object -->

    <owl:Class rdf:about="http://www.ics.forth.gr/isl/CRMdig/D29_Annotation_Object">
        <rdfs:subClassOf rdf:resource="http://www.cidoc-crm.org/cidoc-crm/E89_Propositional_Object"/>
        <rdfs:comment xml:lang="en">This class comprises objects that make propositions about other artefacts. 
	Instances of this class are not the attributes themselves, by which things are annotated, 
	but represent the connection between the concepts related in a proposition, and the activities of creation, modification and deletion. 
	</rdfs:comment>
    </owl:Class>
    


    <!-- http://www.ics.forth.gr/isl/CRMdig/D2_Digitization_Process -->

    <owl:Class rdf:about="http://www.ics.forth.gr/isl/CRMdig/D2_Digitization_Process">
        <rdfs:subClassOf rdf:resource="http://www.ics.forth.gr/isl/CRMdig/D11_Digital_Measurement_Event"/>
        <rdfs:comment xml:lang="en">This class comprises events that result in the creation of instances of D9 Data Object that 
	represent the appearance and/or form of an instance of E18 Physical Thing such as paper documents, statues, buildings, paintings, etc. 
	A particular case is the analogue-to-digital conversion of audiovisual material.
	This class represents the transition from a material thing to an immaterial representation of it. 
	The characteristic subsequent processing steps on digital objects are regarded as instances of D3 Formal Derivation.
</rdfs:comment>
        <rdfs:isDefinedBy rdf:resource="http://www.ics.forth.gr/isl/CRMdig/"/>
    </owl:Class>
    


    <!-- http://www.ics.forth.gr/isl/CRMdig/D7_Digital_Machine_Event -->

    <owl:Class rdf:about="http://www.ics.forth.gr/isl/CRMdig/D7_Digital_Machine_Event"/>
    


    <!-- http://www.ics.forth.gr/isl/CRMdig/D9_Data_Object -->

    <owl:Class rdf:about="http://www.ics.forth.gr/isl/CRMdig/D9_Data_Object">
        <rdfs:subClassOf rdf:resource="http://www.cidoc-crm.org/cidoc-crm/E54_Dimension"/>
        <rdfs:subClassOf rdf:resource="http://www.ics.forth.gr/isl/CRMdig/D1_Digital_Object"/>
        <rdfs:comment xml:lang="en">This class comprises instances of D1 Digital Object that are the direct result of a digital measurement or a formal derivative of it, containing quantitative properties of some physical things or other constellations of matter.</rdfs:comment>
        <rdfs:isDefinedBy rdf:resource="http://www.ics.forth.gr/isl/CRMdig/"/>
    </owl:Class>
    


    <!-- http://www.w3.org/ns/prov#Activity -->

    <owl:Class rdf:about="http://www.w3.org/ns/prov#Activity"/>
    


    <!-- https://w3id.org/cnr-ispc/ontology/branco#CladdingUnit -->

    <owl:Class rdf:about="https://w3id.org/cnr-ispc/ontology/branco#CladdingUnit">
        <rdfs:subClassOf rdf:resource="https://w3id.org/cnr-ispc/ontology/branco#InterpretativeUnit"/>
        <owl:disjointWith rdf:resource="https://w3id.org/cnr-ispc/ontology/branco#StructuralUnit"/>
        <rdfs:comment xml:lang="en">Interpretative Unit can refer to events concerning decorative elements, which covers structural element (e.g. the frescoes decoration on a wall): in this case, it is said &lt;i&gt;cladding unit&lt;/i&gt;</rdfs:comment>
        <rdfs:isDefinedBy rdf:resource="https://w3id.org/cnr-ispc/ontology/branco#"/>
    </owl:Class>
    


    <!-- https://w3id.org/cnr-ispc/ontology/branco#Interpretation -->

    <owl:Class rdf:about="https://w3id.org/cnr-ispc/ontology/branco#Interpretation">
        <rdfs:subClassOf rdf:resource="http://purl.org/emmedi/hico/InterpretationAct"/>
        <rdfs:subClassOf rdf:resource="http://www.cidoc-crm.org/cidoc-crm/E13_Attribute_Assignment"/>
        <rdfs:comment xml:lang="en">This class comprises interpretative acts, with which different properties (defined as instances of class &lt;code&gt;crm:E55_Type&lt;/code&gt;) are associated to a cultural object or site on the basis of a scientific analysis, relying on different sources and supported by several criteria.</rdfs:comment>
        <rdfs:isDefinedBy rdf:resource="https://w3id.org/cnr-ispc/ontology/branco#"/>
    </owl:Class>
    


    <!-- https://w3id.org/cnr-ispc/ontology/branco#InterpretativeUnit -->

    <owl:Class rdf:about="https://w3id.org/cnr-ispc/ontology/branco#InterpretativeUnit">
        <rdfs:subClassOf rdf:resource="http://www.cidoc-crm.org/cidoc-crm/E89_Propositional_Object"/>
        <rdfs:comment xml:lang="en">The interpretative unit is the core unit of a reconstruction activity. Based on the archeological concept of &lt;i&gt;stratigraphic unit&lt;/i&gt;, the interpretative unit tries to extend the semantics of this concept also to non-archeological sites. It models an event of destruction (&lt;code&gt;crm:6_Destruction&lt;/code&gt;) or modification (&lt;code&gt;crm:E11_Modification&lt;/code&gt; and its subclasses) on a physical object.</rdfs:comment>
        <rdfs:isDefinedBy rdf:resource="https://w3id.org/cnr-ispc/ontology/branco#"/>
    </owl:Class>
    


    <!-- https://w3id.org/cnr-ispc/ontology/branco#Reconstruction -->

    <owl:Class rdf:about="https://w3id.org/cnr-ispc/ontology/branco#Reconstruction">
        <rdfs:subClassOf rdf:resource="http://www.cidoc-crm.org/cidoc-crm/E89_Propositional_Object"/>
        <rdfs:comment xml:lang="en">A reconstruction is a system of interpretative units which, on the basis of scrupulous and scientific research, describe the original appearance of a cultural site or artwork</rdfs:comment>
        <rdfs:isDefinedBy rdf:resource="https://w3id.org/cnr-ispc/ontology/branco#"/>
    </owl:Class>
    


    <!-- https://w3id.org/cnr-ispc/ontology/branco#SemanticNode -->

    <owl:Class rdf:about="https://w3id.org/cnr-ispc/ontology/branco#SemanticNode">
        <rdfs:subClassOf rdf:resource="http://www.ics.forth.gr/isl/CRMdig/D29_Annotation_Object"/>
        <rdfs:comment xml:lang="en">This class comprises all the annotation objects which may embedded in a 3D Model to add semantics annotation. For the implementation of semantic nodes in the framework &lt;a href=&quot;https://osiris.itabc.cnr.it/aton/&quot;&gt;ATON&lt;/a&gt;, see the reference &lt;a href=&quot;https://aton.ispc.cnr.it/apidoc/client/Node.html&quot;&gt;documentation page&lt;/a&gt;</rdfs:comment>
        <rdfs:isDefinedBy rdf:resource="https://w3id.org/cnr-ispc/ontology/branco#"/>
    </owl:Class>
    


    <!-- https://w3id.org/cnr-ispc/ontology/branco#StructuralUnit -->

    <owl:Class rdf:about="https://w3id.org/cnr-ispc/ontology/branco#StructuralUnit">
        <rdfs:subClassOf rdf:resource="https://w3id.org/cnr-ispc/ontology/branco#InterpretativeUnit"/>
        <rdfs:comment xml:lang="en">Interpretative Unit can refer to events concerning structural elements, considered without any decoration: in this case, it is said &lt;i&gt;structural unit&lt;/i&gt;</rdfs:comment>
        <rdfs:isDefinedBy rdf:resource="https://w3id.org/cnr-ispc/ontology/branco#"/>
    </owl:Class>
    


    <!-- 
    ///////////////////////////////////////////////////////////////////////////////////////
    //
    // Individuals
    //
    ///////////////////////////////////////////////////////////////////////////////////////
     -->

    


    <!-- https://w3id.org/cnr-ispc/ontology/branco#archival-source -->

    <owl:NamedIndividual rdf:about="https://w3id.org/cnr-ispc/ontology/branco#archival-source">
        <rdf:type rdf:resource="http://purl.org/emmedi/hico/InterpretationCriterion"/>
        <rdfs:comment xml:lang="en">This individual refers to a interpretative criterion (&lt;code&gt;hico:InterpretationCriterion&lt;/code&gt;): the consultation of archival documents</rdfs:comment>
        <rdfs:isDefinedBy rdf:resource="https://w3id.org/cnr-ispc/ontology/branco#"/>
    </owl:NamedIndividual>
    


    <!-- https://w3id.org/cnr-ispc/ontology/branco#author -->

    <owl:NamedIndividual rdf:about="https://w3id.org/cnr-ispc/ontology/branco#author">
        <rdf:type rdf:resource="http://www.cidoc-crm.org/cidoc-crm/E55_Type"/>
        <rdfs:comment>This individual refers to a type of features which may be assigned during an interpretation, i.e. the author (suggested type: &lt;code&gt;crm:E39_Actor&lt;/code&gt; or its subclasses).</rdfs:comment>
        <rdfs:isDefinedBy rdf:resource="https://w3id.org/cnr-ispc/ontology/branco#"/>
    </owl:NamedIndividual>
    


    <!-- https://w3id.org/cnr-ispc/ontology/branco#commission -->

    <owl:NamedIndividual rdf:about="https://w3id.org/cnr-ispc/ontology/branco#commission">
        <rdf:type rdf:resource="http://www.cidoc-crm.org/cidoc-crm/E55_Type"/>
        <rdfs:comment>This individual refers to a type of features which may be assigned during an interpretation, i.e. the actor who commissioned the artwork or monument (suggested type: &lt;code&gt;crm:E39_Actor&lt;/code&gt; or its subclasses).</rdfs:comment>
        <rdfs:isDefinedBy rdf:resource="https://w3id.org/cnr-ispc/ontology/branco#"/>
    </owl:NamedIndividual>
    


    <!-- https://w3id.org/cnr-ispc/ontology/branco#comparison -->

    <owl:NamedIndividual rdf:about="https://w3id.org/cnr-ispc/ontology/branco#comparison">
        <rdf:type rdf:resource="http://purl.org/emmedi/hico/InterpretationCriterion"/>
        <rdfs:comment xml:lang="en">This individual refers to a interpretative criterion (&lt;code&gt;hico:InterpretationCriterion&lt;/code&gt;): the comparison with similar objects (they can be asserted via &lt;code&gt;:providesComparisonWith&lt;/code&gt;)</rdfs:comment>
        <rdfs:isDefinedBy rdf:resource="https://w3id.org/cnr-ispc/ontology/branco#"/>
    </owl:NamedIndividual>
    


    <!-- https://w3id.org/cnr-ispc/ontology/branco#diagnostic-data -->

    <owl:NamedIndividual rdf:about="https://w3id.org/cnr-ispc/ontology/branco#diagnostic-data">
        <rdf:type rdf:resource="http://purl.org/emmedi/hico/InterpretationCriterion"/>
        <rdfs:comment xml:lang="en">This individual refers to a interpretative criterion (&lt;code&gt;hico:InterpretationCriterion&lt;/code&gt;): scientific evidence derived from diagnostic data acquired through physico-chemical analyses</rdfs:comment>
        <rdfs:isDefinedBy rdf:resource="https://w3id.org/cnr-ispc/ontology/branco#"/>
    </owl:NamedIndividual>
    


    <!-- https://w3id.org/cnr-ispc/ontology/branco#dimension -->

    <owl:NamedIndividual rdf:about="https://w3id.org/cnr-ispc/ontology/branco#dimension">
        <rdf:type rdf:resource="http://www.cidoc-crm.org/cidoc-crm/E55_Type"/>
        <rdfs:comment xml:lang="en">This individual refers to a type of features which may be assigned during an interpretation, i.e. the dimension of the object (suggested type: &lt;code&gt;crm:E54_Dimension&lt;/code&gt;. The numerical value can be asserted also as an &lt;code&gt;xsd:float&lt;/code&gt;, as indicated in &lt;a href=&quot;https://www.cidoc-crm.org/sites/default/files/Implementing%20the%20CIDOC%20Conceptual%20Reference%20Model%20in%20RDF.pdf&quot;&gt;&lt;i&gt;Implementing the CIDOC Conceptual
Reference Model in RDF&lt;/i&gt;&lt;/a&gt;, v.1.0).</rdfs:comment>
        <rdfs:isDefinedBy rdf:resource="https://w3id.org/cnr-ispc/ontology/branco#"/>
    </owl:NamedIndividual>
    


    <!-- https://w3id.org/cnr-ispc/ontology/branco#general-rule -->

    <owl:NamedIndividual rdf:about="https://w3id.org/cnr-ispc/ontology/branco#general-rule">
        <rdf:type rdf:resource="http://purl.org/emmedi/hico/InterpretationCriterion"/>
        <rdfs:comment xml:lang="en">This individual refers to a interpretative criterion (&lt;code&gt;hico:InterpretationCriterion&lt;/code&gt;): general rules (such as the proportion in the dimensions of temples in Greco-Roman architecture)</rdfs:comment>
        <rdfs:isDefinedBy rdf:resource="https://w3id.org/cnr-ispc/ontology/branco#"/>
    </owl:NamedIndividual>
    


    <!-- https://w3id.org/cnr-ispc/ontology/branco#iconography -->

    <owl:NamedIndividual rdf:about="https://w3id.org/cnr-ispc/ontology/branco#iconography">
        <rdf:type rdf:resource="http://www.cidoc-crm.org/cidoc-crm/E55_Type"/>
        <rdfs:comment>This individual refers to a type of features which may be assigned during an interpretation. It refers to the iconography (usually of cladding unit), which pertains to &quot;the identification of such images, stories and allegories&quot; (Panofsky). 

In Branco, the definition of a specific iconography may be asserted as follows: a &lt;code&gt;:Interpretation crm:P141_assigned crm:E36_Visual_Item&lt;/code&gt;. With this axiom, this conceptual model is interoperable with the &lt;a href=&quot;https://ncarboni.github.io/vir/&quot;&gt;VIR - Visual Representation Ontology&lt;/a&gt; and the class &lt;code&gt;IC9 Representation&lt;/code&gt;, which is in turn subclass of &lt;code&gt;crm:E36_Visual_Item&lt;/code&gt;.

Association of an iconography to an Iconclass concept can be asserted as &lt;code&gt;crm:E36_Visual_Item crm:P48_has_preferred_identifier crm:E42_Identifier&lt;/code&gt;</rdfs:comment>
        <rdfs:isDefinedBy rdf:resource="https://w3id.org/cnr-ispc/ontology/branco#"/>
    </owl:NamedIndividual>
    


    <!-- https://w3id.org/cnr-ispc/ontology/branco#location -->

    <owl:NamedIndividual rdf:about="https://w3id.org/cnr-ispc/ontology/branco#location">
        <rdf:type rdf:resource="http://www.cidoc-crm.org/cidoc-crm/E55_Type"/>
        <rdfs:comment xml:lang="en">This individual refers to a type of features which may be assigned during an interpretation. It refers to the location in which the object of an interpretative unit might be found (suggested type: &lt;code&gt;crm:E53_Place&lt;/code&gt;, with specifications asserted via &lt;code&gt;crm:P157_is_at_rest_relative_to&lt;/code&gt;)</rdfs:comment>
        <rdfs:isDefinedBy rdf:resource="https://w3id.org/cnr-ispc/ontology/branco#"/>
    </owl:NamedIndividual>
    


    <!-- https://w3id.org/cnr-ispc/ontology/branco#material -->

    <owl:NamedIndividual rdf:about="https://w3id.org/cnr-ispc/ontology/branco#material">
        <rdf:type rdf:resource="http://www.cidoc-crm.org/cidoc-crm/E55_Type"/>
        <rdfs:comment xml:lang="en">This individual refers to a type of features which may be assigned during an interpretation. It refers to the material of which the studied object is made (suggested type: &lt;code&gt;crm:E57_Material&lt;/code&gt;)</rdfs:comment>
        <rdfs:isDefinedBy rdf:resource="https://w3id.org/cnr-ispc/ontology/branco#"/>
    </owl:NamedIndividual>
    


    <!-- https://w3id.org/cnr-ispc/ontology/branco#observation -->

    <owl:NamedIndividual rdf:about="https://w3id.org/cnr-ispc/ontology/branco#observation">
        <rdf:type rdf:resource="http://purl.org/emmedi/hico/InterpretationCriterion"/>
        <rdfs:comment xml:lang="en">This individual refers to a interpretative criterion (&lt;code&gt;hico:InterpretationCriterion&lt;/code&gt;): direct observation of the studied object</rdfs:comment>
        <rdfs:isDefinedBy rdf:resource="https://w3id.org/cnr-ispc/ontology/branco#"/>
    </owl:NamedIndividual>
    


    <!-- https://w3id.org/cnr-ispc/ontology/branco#provenance -->

    <owl:NamedIndividual rdf:about="https://w3id.org/cnr-ispc/ontology/branco#provenance">
        <rdf:type rdf:resource="http://www.cidoc-crm.org/cidoc-crm/E55_Type"/>
        <rdfs:comment xml:lang="en">This individual refers to a type of features which may be assigned during an interpretation, i.e. the pervious owner of the studied objects (suggested type: &lt;code&gt;crm:E39_Actor&lt;/code&gt; or its subclasses).</rdfs:comment>
        <rdfs:isDefinedBy rdf:resource="https://w3id.org/cnr-ispc/ontology/branco#"/>
    </owl:NamedIndividual>
    


    <!-- https://w3id.org/cnr-ispc/ontology/branco#style -->

    <owl:NamedIndividual rdf:about="https://w3id.org/cnr-ispc/ontology/branco#style">
        <rdf:type rdf:resource="http://www.cidoc-crm.org/cidoc-crm/E55_Type"/>
        <rdfs:comment xml:lang="en">This individual refers to a type of features which may be assigned during an interpretation, i.e. the style in which the object is made. &quot;By style, it is meant the constant form - and sometimes the constant elements, qualities, and expression - in the art of an individual or a group&quot; (Shapiro).

Since single elements may be found, it is recommended the identification of specific features (e.g. drapery) via the axiom &lt;code&gt;:Interpretation cito:citesAsEvidence crm:E26_Physical_Feature&lt;/code&gt;

In CIDOC CRM style, i.e. &quot;a style applicable to all paintings sharing the characteristics of the works produced by the Impressionist painters, regardless of historical context&quot;, defines morphological object types that fall under E55 Type&quot; (from CIDOC CRM documentation, v. 7.1.3, class crm:E4_Period, fifth paragraph).</rdfs:comment>
        <rdfs:isDefinedBy rdf:resource="https://w3id.org/cnr-ispc/ontology/branco#"/>
    </owl:NamedIndividual>
    


    <!-- https://w3id.org/cnr-ispc/ontology/branco#technique -->

    <owl:NamedIndividual rdf:about="https://w3id.org/cnr-ispc/ontology/branco#technique">
        <rdf:type rdf:resource="http://www.cidoc-crm.org/cidoc-crm/E55_Type"/>
        <rdfs:comment xml:lang="en">This individual refers to a type of features which may be assigned during an interpretation. It refers to the technique used for the production of the studied object (suggested type: &lt;code&gt;crm:E55_Type&lt;/code&gt;)</rdfs:comment>
        <rdfs:isDefinedBy rdf:resource="https://w3id.org/cnr-ispc/ontology/branco#"/>
    </owl:NamedIndividual>
    


    <!-- 
    ///////////////////////////////////////////////////////////////////////////////////////
    //
    // General axioms
    //
    ///////////////////////////////////////////////////////////////////////////////////////
     -->

    <rdf:Description>
        <rdf:type rdf:resource="http://www.w3.org/2002/07/owl#AllDisjointClasses"/>
        <owl:members rdf:parseType="Collection">
            <rdf:Description rdf:about="http://www.cidoc-crm.org/cidoc-crm/E12_Production"/>
            <rdf:Description rdf:about="http://www.cidoc-crm.org/cidoc-crm/E79_Part_Addition"/>
            <rdf:Description rdf:about="http://www.cidoc-crm.org/cidoc-crm/E80_Part_Removal"/>
        </owl:members>
    </rdf:Description>
    <rdf:Description>
        <rdf:type rdf:resource="http://www.w3.org/2002/07/owl#AllDisjointClasses"/>
        <owl:members rdf:parseType="Collection">
            <rdf:Description rdf:about="http://www.cidoc-crm.org/cidoc-crm/E18_Physical_Thing"/>
            <rdf:Description rdf:about="http://www.ics.forth.gr/isl/CRMdig/D2_Digitization_Process"/>
            <rdf:Description rdf:about="http://www.ics.forth.gr/isl/CRMdig/D9_Data_Object"/>
            <rdf:Description rdf:about="https://w3id.org/cnr-ispc/ontology/branco#InterpretativeUnit"/>
            <rdf:Description rdf:about="https://w3id.org/cnr-ispc/ontology/branco#Reconstruction"/>
            <rdf:Description rdf:about="https://w3id.org/cnr-ispc/ontology/branco#SemanticNode"/>
        </owl:members>
    </rdf:Description>
</rdf:RDF>



<!-- Generated by the OWL API (version 4.2.5.20160517-0735) https://github.com/owlcs/owlapi -->

